
x_i(t) \in \{-1, +1 \}


w_i(1) = 1 \forall i


\hat{z}(1) = sign(\sum_i x_i(0))


w_i(2) = [ x_i(1) = z(1)] w_i(1)


\hat{z}(2) = sign(\sum_i w_i(2) x_i(2))

w_i(t+1) = [ x_i(t) = z(t)] w_i(t)

\hat{z}(t) = sign(\sum_i w_i(t) x_i(t))

L(t) = \# \text{ Losses on days 1...} t\\
= \sum_{t'=1}^t[\hat{z}(t' = z(t)]


\lim_{t\rightarrow\infty} L(t) \leq \log_2(n)



w_i(t+1) =
\left\{
  \begin{array}{ll}
    1  & \mbox{if } z(t) = x_i(t)\\
    \alpha  & \mbox{if } z(t) \not= x_i(t)
  \end{array}
\right\}w_i(t)

w_*(t) \geq \alpha^n \indent \forall t

w(t) =\sum_i w_i(t)

w \downarrow \frac{\alpha + 1}{2}


w(1) = n

w(t) \leq n ( \frac{\alpha +1}{2})^l

w(t) \geq \alpha^m \indent \forall t



n ( \frac{\alpha +1}{2})^l \geq w(t) \geq \alpha^m \indent \forall t


l\log(\frac{\alpha +1}{2})) \geq m\log(\alpha) -\log(n)


1 \leq \frac{ m\log(\alpha) - \log(n)}{\log(\frac{\alpha +1}{2})}

w_i(t+1) = w_i(t) - \zeta\frac{\delta \hat{E}}{\delta w_i}

E = \lambda\frac{1}{2}(w-w^*)^2 \indent w^* = 0 \text{ (just to make things easier)}

w_i(t+1) = w_i(t) - \zeta\frac{\delta \hat{E}}{\delta w_i}\\
=(1-\zeta\lambda)w(t)

w_i(t) =(1-\zeta\lambda)^tw(0)

|1-\zeta\lambda|<1

-1< 1-\zeta\lambda <1


-2 <-\zeta\lambda < 0\\
0 < \zeta\lambda < 2\\
0 < \zeta\lambda < \frac{2}{\lambda}
